Structural substitution overhauled. Checkpoint.

theories/StructuralFreeVariables.v
@@ -2,6 +2,7 @@ From Coq Require Export
   Lists.List.
 Export ListNotations.
 From Lang Require Import
+  InTactics
   Invert
   Terms.
 
@@ -14,26 +15,56 @@ Fixpoint remove_all x li :=
   end.
 (* tail-recursive version flips the order *)
 
-Theorem in_remove_all : forall x li,
+Lemma in_remove_all : forall x li,
   ~In x (remove_all x li).
 Proof.
   intros x li C. generalize dependent x. induction li; intros; simpl in *. { destruct C. }
   destruct (eqb_spec x a). { apply IHli in C as []. } destruct C. { subst. apply n. reflexivity. } apply IHli in H as [].
 Qed.
 
-Theorem in_remove_all_neq : forall x y li,
+Lemma in_remove_all_neq : forall x y li,
   x <> y ->
   (In x (remove_all y li) <-> In x li).
 Proof.
   intros x y li H. generalize dependent x. generalize dependent y. induction li; intros; simpl in *. { split; intros []. }
   destruct (eqb_spec y a).
   - subst. split; intros.
-    + right. eapply IHli. { apply H. } assumption.
+    + right. eapply IHli; eassumption.
     + destruct H0. { subst. contradiction H. reflexivity. } apply IHli; assumption.
-  - split; intros H0; (destruct H0; [left; assumption |]; right; eapply IHli; [apply H | assumption]).
+  - split; intros H0; (destruct H0; [left; assumption |]; right; eapply IHli; eassumption).
 Qed.
 
-Fixpoint structural_fv t :=
+Lemma remove_all_app : forall x a b,
+  remove_all x (a ++ b) = remove_all x a ++ remove_all x b.
+Proof.
+  intros x a. generalize dependent x. induction a; intros; simpl in *. { reflexivity. }
+  destruct (eqb_spec x a). { apply IHa. } simpl. f_equal. apply IHa.
+Qed.
+
+Lemma rev_remove_all : forall x li,
+  rev (remove_all x li) = remove_all x (rev li).
+Proof.
+  intros. generalize dependent x. induction li; intros; simpl in *. { reflexivity. }
+  rewrite remove_all_app. simpl. destruct (eqb x a). { rewrite app_nil_r. apply IHli. } simpl. f_equal. apply IHli.
+Qed.
+
+Lemma remove_all_swap : forall x y li,
+  remove_all x (remove_all y li) = remove_all y (remove_all x li).
+Proof.
+  intros. generalize dependent x. generalize dependent y. induction li; intros; simpl in *. { reflexivity. }
+  destruct (eqb_spec y a). { subst. destruct (eqb_spec x a). { subst. reflexivity. } simpl. rewrite eqb_refl. apply IHli. }
+  destruct (eqb_spec x a). { subst. simpl. rewrite eqb_refl. apply IHli. }
+  simpl. apply eqb_neq in n. apply eqb_neq in n0. rewrite n. rewrite n0. f_equal. apply IHli.
+Qed.
+
+Lemma remove_all_shadow : forall x li,
+  remove_all x (remove_all x li) = remove_all x li.
+Proof.
+  intros. generalize dependent x. induction li; intros; simpl in *. { reflexivity. }
+  destruct (eqb x a) eqn:E. { apply IHli. } simpl. rewrite E. f_equal. apply IHli.
+Qed.
+
+Fixpoint structural_fv_slow t :=
   match t with
   | TmVoid
   | TmStar _
@@ -42,11 +73,11 @@ Fixpoint structural_fv t :=
   | TmVarS s =>
       [s]
   | TmAppl f x =>
-      structural_fv f ++ structural_fv x
+      structural_fv_slow f ++ structural_fv_slow x
   | TmPack _ arg ty curry
   | TmForA arg ty curry =>
-      structural_fv ty ++ (
-        let recursed := structural_fv curry in
+      structural_fv_slow ty ++ (
+        let recursed := structural_fv_slow curry in
         match arg with
         | None => recursed
         | Some a => remove_all a recursed
@@ -54,68 +85,125 @@ Fixpoint structural_fv t :=
   end.
 
 (* Crucial distinction from an easier-to-implement algorithm! *)
-Example structural_fv_permits_shadowing : forall x,
+Example structural_fv_slow_permits_shadowing : forall x,
   (* Equivalent to `\x. \x. x x`, where the `x`s are distinct and pushed/popped in order. *)
-  structural_fv (TmForA (Some x) TmVoid (TmForA (Some x) TmVoid (TmAppl (TmVarS x) (TmVarS x)))) = [].
+  structural_fv_slow (
+    TmForA (Some x) TmVoid (
+      TmForA (Some x) TmVoid (
+        TmAppl (TmVarS x) (TmVarS x)))) = [].
 Proof. intros. simpl. repeat rewrite eqb_refl. reflexivity. Qed.
 
-(* Crucial distinction from an easier-to-implement algorithm! *)
-Example structural_fv_permits_interrupted_shadowing : forall x y, y <> x ->
+Example structural_fv_slow_permits_interrupted_shadowing : forall x y,
   (* Equivalent to `\x. \y. \x. x x`, where the `x`s are distinct and pushed/popped in order. *)
-  structural_fv (TmForA (Some x) TmVoid (TmForA (Some y) TmVoid (TmForA (Some x) TmVoid (TmAppl (TmVarS x) (TmVarS x))))) = [].
+  structural_fv_slow (
+    TmForA (Some x) TmVoid (
+      TmForA (Some y) TmVoid (
+        TmForA (Some x) TmVoid (
+          TmAppl (TmVarS x) (TmVarS x))))) = [].
 Proof. intros. simpl. rewrite eqb_refl. reflexivity. Qed.
 
 Example structural_fv_respects_scope : forall x,
   (* Equivalent to `(\x:0. 0) x`, in which the outer `x` is still free *)
-  structural_fv (TmAppl (TmForA (Some x) TmVoid TmVoid) (TmVarS x)) = [x].
+  structural_fv_slow (TmAppl (TmForA (Some x) TmVoid TmVoid) (TmVarS x)) = [x].
 Proof. intros. simpl. reflexivity. Qed.
 
-(*
-Fixpoint structural_fv_fast acc t :=
+Fixpoint structural_fv_fast acc shadowed t :=
   match t with
   | TmVoid
   | TmStar _
   | TmAtom _ =>
       acc
   | TmVarS s =>
-      s :: acc
+      if existsb (eqb s) shadowed then acc else s :: acc
   | TmPack _ None a b
   | TmForA None a b
   | TmAppl a b =>
-      structural_fv_fast (structural_fv_fast acc b) a
+      structural_fv_fast (structural_fv_fast acc shadowed a) shadowed b
   | TmPack _ (Some arg) ty curry
   | TmForA (Some arg) ty curry =>
-      structural_fv_fast (remove_if_head arg (structural_fv_fast acc curry)) ty
+      structural_fv_fast (structural_fv_fast acc shadowed ty) (arg :: shadowed) curry
   end.
+
+Definition structural_fv t := rev' (structural_fv_fast [] [] t).
+Arguments structural_fv/ t.
 
 (* Crucial distinction from an easier-to-implement algorithm! *)
 Example structural_fv_fast_permits_shadowing : forall x,
   (* Equivalent to `\x. \x. x x`, where the `x`s are distinct and pushed/popped in order. *)
-  structural_fv_fast [] (TmForA (Some x) TmVoid (TmForA (Some x) TmVoid (TmAppl (TmVarS x) (TmVarS x)))) = [].
+  structural_fv (
+    TmForA (Some x) TmVoid (
+      TmForA (Some x) TmVoid (
+        TmAppl (TmVarS x) (TmVarS x)))) = [].
 Proof. intros. simpl. repeat rewrite eqb_refl. reflexivity. Qed.
 
-(* Crucial distinction from an easier-to-implement algorithm! *)
-Example structural_fv_fast_permits_interrupted_shadowing : forall x y, y <> x ->
+Example structural_fv_fast_permits_interrupted_shadowing : forall x y,
   (* Equivalent to `\x. \y. \x. x x`, where the `x`s are distinct and pushed/popped in order. *)
-  structural_fv_fast [] (TmForA (Some x) TmVoid (TmForA (Some y) TmVoid (TmForA (Some x) TmVoid (TmAppl (TmVarS x) (TmVarS x))))) = [].
-Proof. intros. apply eqb_neq in H. simpl. rewrite eqb_refl. rewrite H. rewrite eqb_refl. reflexivity. Qed.
+  structural_fv (
+    TmForA (Some x) TmVoid (
+      TmForA (Some y) TmVoid (
+        TmForA (Some x) TmVoid (
+          TmAppl (TmVarS x) (TmVarS x))))) = [].
+Proof. intros. simpl. rewrite eqb_refl. reflexivity. Qed.
 
 Example structural_fv_fast_respects_scope : forall x,
   (* Equivalent to `(\x:0. 0) x`, in which the outer `x` is still free *)
-  structural_fv_fast [] (TmAppl (TmForA (Some x) TmVoid TmVoid) (TmVarS x)) = [x].
-Proof. intros. simpl. Abort.
+  structural_fv (TmAppl (TmForA (Some x) TmVoid TmVoid) (TmVarS x)) = [x].
+Proof. intros. reflexivity. Qed.
 
-Theorem structural_fv_fast_slow_eq : forall t,
-  structural_fv_slow t = rev (snd (structural_fv_fast [] [] t)).
+Lemma structural_fv_fast_acc : forall hd tl shadowed t,
+  structural_fv_fast (hd ++ tl) shadowed t = structural_fv_fast hd shadowed t ++ tl.
 Proof.
-  intros t. induction t; intros; simpl in *; try reflexivity.
-  - destruct arg.
-    + destruct (structural_fv_slow t2).
-      * rewrite app_nil_r. rewrite IHt1. destruct (structural_fv_fast [] [] t1).
+  intros. generalize dependent hd. generalize dependent tl. generalize dependent shadowed.
+  induction t; intros; simpl in *; try reflexivity;
+  [destruct (existsb (eqb id) shadowed); reflexivity | destruct arg | destruct arg |];
+  rewrite IHt1; rewrite IHt2; reflexivity.
 Qed.
 
-Definition structural_fv := structural_fv_fast [].
-*)
+Lemma fold_left_rm_nil : forall shadowed,
+  fold_left (fun li x => remove_all x li) shadowed [] = [].
+Proof. induction shadowed. { reflexivity. } assumption. Qed.
+
+Lemma fold_left_rm_app : forall a b rm,
+  let f := fun li x => remove_all x li in
+  fold_left f rm a ++ fold_left f rm b = fold_left f rm (a ++ b).
+Proof.
+  intros. unfold f. clear f. generalize dependent b. generalize dependent a.
+  induction rm; intros; simpl in *. { reflexivity. } rewrite remove_all_app. apply IHrm.
+Qed.
+
+Lemma structural_fv_fast_shadowed : forall acc shadowed t,
+  structural_fv_fast acc shadowed t = fold_left (fun li x => remove_all x li) shadowed (structural_fv_fast [] [] t) ++ acc.
+Proof.
+  intros. generalize dependent acc. generalize dependent shadowed.
+  induction t; intros; simpl in *; try rewrite fold_left_rm_nil; try reflexivity.
+  - destruct (existsb_in eqb id shadowed eqb_spec).
+    + induction shadowed; destruct i; simpl; [subst; rewrite eqb_refl | destruct (eqb_spec a id)];
+      try (rewrite fold_left_rm_nil; reflexivity). apply IHshadowed. assumption.
+    + induction shadowed; simpl in *. { reflexivity. }
+      apply Decidable.not_or in n as [Ha H]. apply eqb_neq in Ha. rewrite Ha. apply IHshadowed. assumption.
+  - destruct arg; simpl in *; rewrite IHt1; rewrite IHt2; rewrite app_assoc; f_equal.
+    + rewrite (structural_fv_fast_acc [] (structural_fv_fast [] [] t1)). rewrite <- fold_left_rm_app. f_equal.
+      rewrite (IHt2 [s]). simpl. rewrite app_nil_r. reflexivity.
+    + rewrite (structural_fv_fast_acc [] (structural_fv_fast [] [] t1)). apply fold_left_rm_app.
+  - destruct arg; simpl in *; rewrite IHt1; rewrite IHt2; rewrite app_assoc; f_equal.
+    + rewrite (structural_fv_fast_acc [] (structural_fv_fast [] [] t1)). rewrite <- fold_left_rm_app. f_equal.
+      rewrite (IHt2 [s]). simpl. rewrite app_nil_r. reflexivity.
+    + rewrite (structural_fv_fast_acc [] (structural_fv_fast [] [] t1)). apply fold_left_rm_app.
+  - rewrite IHt1. rewrite IHt2. rewrite app_assoc. f_equal.
+    rewrite (structural_fv_fast_acc [] (structural_fv_fast [] [] t1)). apply fold_left_rm_app.
+Qed.
+
+Theorem structural_fv_fast_slow : forall t,
+  structural_fv t = structural_fv_slow t.
+Proof.
+  intros. simpl in *. unfold rev'. rewrite <- rev_alt. induction t; intros; simpl in *; try reflexivity.
+  - destruct arg; rewrite (structural_fv_fast_acc [] (structural_fv_fast [] [] t1)); rewrite rev_app_distr; rewrite IHt1;
+    [rewrite structural_fv_fast_shadowed; rewrite app_nil_r; simpl; rewrite rev_remove_all |]; rewrite IHt2; reflexivity.
+  - destruct arg; rewrite (structural_fv_fast_acc [] (structural_fv_fast [] [] t1)); rewrite rev_app_distr; rewrite IHt1;
+    [rewrite structural_fv_fast_shadowed; rewrite app_nil_r; simpl; rewrite rev_remove_all |]; rewrite IHt2; reflexivity.
+  - rewrite (structural_fv_fast_acc [] (structural_fv_fast [] [] t1)).
+    rewrite rev_app_distr. rewrite IHt1. rewrite IHt2. reflexivity.
+Qed.
 
 Inductive Wherever {T} (x : T) : list T -> list T -> Prop :=
   | WhereverNil :
@@ -205,7 +293,7 @@ Qed.
 Theorem reflect_structural_fv : forall t v,
   structural_fv t = v <-> StructurallyFreeIn t v.
 Proof.
-  split; intros.
+  intros. rewrite structural_fv_fast_slow. split; intros.
   - generalize dependent v. induction t; intros; subst; simpl in *; try constructor;
     econstructor; try apply IHt1; try apply IHt2; try reflexivity;
     (destruct arg; [| reflexivity]); apply wherever_remove_all; reflexivity.
