theories/HoleStack.v
@@ -1,0 +1,18 @@
+From Lang Require Import
+  Hole
+  StructuralHole
+  Terms.
+
+Print hole.
+Inductive hole_stack : Set :=
+  | HoleStackHere
+  | HoleStackPack (id : string) (arg : option string) (ty : structural_hole) (curry : list hole_stack)
+  | HoleStackForA (arg : option string) (ty : structural_hole) (body : list hole_stack)
+  | HoleStackAppl (f : list hole_stack) (x : list hole_stack)
+  .
+
+Fixpoint first_hole h :=
+  match h with
+  | HoleStackHere => SHoleHere
+  | HoleStackPack id arg ty curry => SHolePack id arg ty (hd curry)
+  end.
